Store free list in pool data type
This means that indices will be used contiguously before expanding the
number of indices used, which will be useful when switching indices from
Nats to u32s in the future.

Valaig/Aig/Basic.lean
@@ -28,6 +28,14 @@ end Input
 -/
 abbrev InputData := { input : Input // input.var ≠ .constant }
 
+namespace InputData
+
+@[inline]
+instance : Inhabited InputData where
+  default := ⟨{ var := Var.constant + 1 }, by grind⟩
+
+end InputData
+
 /--
   The metadata of a latch in the Aig.
 -/
@@ -46,6 +54,14 @@ end Latch
   NOTE: Users should not rely on this type, it may change!
 -/
 abbrev LatchData := { latch : Latch // latch.var ≠ .constant }
+
+namespace LatchData
+
+@[inline]
+instance : Inhabited LatchData where
+  default := ⟨{ var := Var.constant + 1, next := .false, reset := none }, by grind⟩
+
+end LatchData
 
 end Valaig.Aig
 
@@ -202,10 +218,10 @@ structure Aig where
   private _nodes : Aig.NodeArray
 
   /-- A mapping from input indices (`InputIdx`) to their definition. -/
-  private _inputs : Pool Aig.InputData
+  _inputs : Pool Aig.InputData
 
   /-- A mapping from latch indices (`LatchIdx`) to their definition. -/
-  private _latches : Pool Aig.LatchData
+  _latches : Pool Aig.LatchData
 
 variable {aig : Aig}
 
@@ -679,7 +695,7 @@ set_option linter.unusedVariables false in
 -/
 @[inline]
 def setNext (idx : LatchIdx) (aig : Aig) (next : Lit) (valid : idx.validIn aig := by grind) : Aig :=
-  { aig with _latches := aig._latches.modify idx.idx (⟨{ ·.val with next }, by grind⟩) }
+  { aig with _latches := aig._latches.modify idx.idx (⟨{ ·.val with next }, by grind⟩) valid }
 
 /--
   Update the next state function for a latch in the Aig.
@@ -697,7 +713,7 @@ set_option linter.unusedVariables false in
 -/
 @[inline]
 def setReset (idx : LatchIdx) (aig : Aig) (reset : Option Lit) (valid : idx.validIn aig := by grind) : Aig :=
-  { aig with _latches := aig._latches.modify idx.idx (⟨{ ·.val with reset }, by grind⟩) }
+  { aig with _latches := aig._latches.modify idx.idx (⟨{ ·.val with reset }, by grind⟩) valid }
 
 /--
   Update the reset function for a latch in the Aig.
@@ -813,20 +829,28 @@ private def setNode (aig : Aig) (var : Var) (node : NodeData) (valid : var.valid
   { aig with _nodes := aig._nodes.set var node.fst node.snd }
 
 @[always_inline]
-private def insertInput (aig : Aig) (idx : InputIdx) (input : Input) (h : input.var ≠ .constant := by grind) : Aig :=
-  { aig with _inputs := aig._inputs.insert idx.idx ⟨input, h⟩ }
+private def pushInput (aig : Aig) (input : Input) (h : input.var ≠ .constant := by grind) : Aig :=
+  { aig with _inputs := aig._inputs.push ⟨input, h⟩ }
 
 @[always_inline]
-private def insertLatch (aig : Aig) (idx : LatchIdx) (latch : Latch) (h : latch.var ≠ .constant := by grind) : Aig :=
-  { aig with _latches := aig._latches.insert idx.idx ⟨latch, h⟩ }
+private def pushLatch (aig : Aig) (latch : Latch) (h : latch.var ≠ .constant := by grind) : Aig :=
+  { aig with _latches := aig._latches.push ⟨latch, h⟩ }
 
 @[always_inline]
-private def eraseInput (aig : Aig) (idx : InputIdx) : Aig :=
-  { aig with _inputs := aig._inputs.erase idx.idx }
+private def eraseInput (aig : Aig) (idx : InputIdx) (valid : idx.validIn aig := by grind) : Aig :=
+  { aig with _inputs := aig._inputs.erase idx.idx valid }
 
 @[always_inline]
-private def eraseLatch (aig : Aig) (idx : LatchIdx) : Aig :=
-  { aig with _latches := aig._latches.erase idx.idx }
+private def eraseLatch (aig : Aig) (idx : LatchIdx) (valid : idx.validIn aig := by grind) : Aig :=
+  { aig with _latches := aig._latches.erase idx.idx valid }
+
+@[always_inline]
+private def moveInput (aig : Aig) (old new : InputIdx) (valid : old.validIn aig := by grind) (notvalid : ¬new.validIn aig ∨ new = old := by grind) : Aig :=
+  { aig with _inputs := aig._inputs.move old.idx new.idx valid (by grind [InputIdx.validIn]) }
+
+@[always_inline]
+private def moveLatch (aig : Aig) (old new : LatchIdx) (valid : old.validIn aig := by grind) (notvalid : ¬new.validIn aig ∨ new = old := by grind) : Aig :=
+  { aig with _latches := aig._latches.move old.idx new.idx valid (by grind [LatchIdx.validIn]) }
 
 attribute [local grind] InputIdx.validIn LatchIdx.validIn newInputIdx newLatchIdx
 
@@ -838,8 +862,8 @@ set_option linter.unusedVariables false in
 def addInput (aig : Aig) : Aig × InputIdx :=
   let idx := aig.newInputIdx
   let var := aig.nextVar
-  let aig := aig.pushNode <| .input idx var
-  let aig := aig.insertInput idx { var }
+  let aig := aig.pushNode <| .input aig.newInputIdx var
+  let aig := aig.pushInput { var }
   (aig, idx)
 
 /--
@@ -853,7 +877,7 @@ def addLatch (aig : Aig) (next : Lit) (reset : Option Lit := none) : Aig × Latc
   let idx := aig.newLatchIdx
   let var := aig.nextVar
   let aig := aig.pushNode <| .latch idx var
-  let aig := aig.insertLatch idx { var, next, reset }
+  let aig := aig.pushLatch { var, next, reset }
   (aig, idx)
 
 /--
@@ -878,8 +902,8 @@ def InputIdx.convertToLatch (idx : InputIdx) (aig : Aig) (next : Lit) (reset : O
   let var := idx.getVar aig
   let latch := aig.newLatchIdx
   let aig := aig.setNode var <| .latch latch var
-  let aig := aig.eraseInput idx
-  let aig := aig.insertLatch latch { var, next, reset } (by grind [getVar])
+  let aig := aig.pushLatch { var, next, reset } (by grind [getVar])
+  let aig := aig.eraseInput idx (by grind [pushLatch, setNode])
   (aig, latch)
 
 /--
@@ -903,7 +927,7 @@ def InputIdx.convertToAnd (idx : InputIdx) (aig : Aig) (rhs0 rhs1 : Lit)
     (varValid : (idx.getVar aig).validIn aig := by grind) : Aig :=
   let var := idx.getVar aig
   let aig := aig.setNode var <| .and rhs0 rhs1
-  let aig := aig.eraseInput idx
+  let aig := aig.eraseInput idx (by grind [setNode])
   aig
 
 /--
@@ -929,10 +953,8 @@ def InputIdx.changeIdx (old new : InputIdx) (aig : Aig)
     (varValid : (old.getVar aig).validIn aig := by grind)
     (unused : ¬new.validIn aig ∨ old = new := by grind) : Aig :=
   let data := aig._inputs[old.idx]
-  let var := data.val.var
-  let aig := aig.setNode data.val.var (.input new data.val.var) (by grind [getVar])
-  let aig := aig.eraseInput old
-  let aig := aig.insertInput new data
+  let aig := aig.moveInput old new
+  let aig := aig.setNode data.val.var (.input new data.val.var) (by grind [getVar, Var.validIn, moveInput])
   aig
 
 /--
@@ -959,8 +981,8 @@ def LatchIdx.convertToInput (idx : LatchIdx) (aig : Aig)
   let var := idx.getVar aig
   let input := aig.newInputIdx
   let aig := aig.setNode var <| .input input var
-  let aig := aig.eraseLatch idx
-  let aig := aig.insertInput input { var } (by grind [getVar])
+  let aig := aig.pushInput { var } (by grind [getVar])
+  let aig := aig.eraseLatch idx (by grind [setNode, pushInput])
   (aig, input)
 
 /--
@@ -984,7 +1006,7 @@ def LatchIdx.convertToAnd (idx : LatchIdx) (aig : Aig) (rhs0 rhs1 : Lit)
     (varValid : (idx.getVar aig).validIn aig := by grind) : Aig :=
   let var := idx.getVar aig
   let aig := aig.setNode var <| .and rhs0 rhs1
-  let aig := aig.eraseLatch idx
+  let aig := aig.eraseLatch idx (by grind [setNode])
   aig
 
 /--
@@ -1010,10 +1032,8 @@ def LatchIdx.changeIdx (old new : LatchIdx) (aig : Aig)
     (varValid : (old.getVar aig).validIn aig := by grind)
     (unused : ¬new.validIn aig ∨ old = new := by grind) : Aig :=
   let data := aig._latches[old.idx]
-  let var := data.val.var
-  let aig := aig.setNode data.val.var (.latch new data.val.var) (by grind [getVar])
-  let aig := aig.eraseLatch old
-  let aig := aig.insertLatch new data
+  let aig := aig.moveLatch old new
+  let aig := aig.setNode data.val.var (.latch new data.val.var) (by grind [getVar, Var.validIn, moveLatch])
   aig
 
 /--
@@ -1041,8 +1061,7 @@ def convertAndToInput (aig : Aig) (var : Var)
     (isAnd : aig[var] matches .and _ _ := by grind) : Aig × InputIdx :=
   let idx := aig.newInputIdx
   let aig := aig.setNode var <| .input idx var
-  let aig := aig.insertInput idx { var }
-    (by simp only [instGetElemVar, instGetElemVar.impl, NodeData.toNode] at isAnd; grind)
+  let aig := aig.pushInput { var } (by simp only [instGetElemVar, instGetElemVar.impl] at isAnd; grind)
   (aig, idx)
 
 /--
@@ -1066,8 +1085,7 @@ def convertAndToLatch (aig : Aig) (var : Var) (next : Lit) (reset : Option Lit :
     (isAnd : aig[var] matches .and _ _ := by grind) : Aig × LatchIdx :=
   let idx := aig.newLatchIdx
   let aig := aig.setNode var <| .latch idx var
-  let aig := aig.insertLatch idx { var, next, reset }
-    (by simp only [instGetElemVar, instGetElemVar.impl, NodeData.toNode] at isAnd; grind)
+  let aig := aig.pushLatch { var, next, reset } (by simp only [instGetElemVar, instGetElemVar.impl] at isAnd; grind)
   (aig, idx)
 
 /--
