Valaig/Data/Pool.lean
@@ -1,10 +1,10 @@
 module
 
-public import Std.Data.HashMap.Basic
-public import Std.Data.HashMap.Iterator
 public import Valaig.Prelude
-import Std.Data.HashMap.IteratorLemmas
-import Std.Data.HashMap.Lemmas
+public import Std.Data.HashSet
+import Std.Data.Iterators.Producers.Range
+import Std.Data.Iterators.Lemmas.Producers.Range
+public import Valaig.ForLean.Array
 
 public section
 namespace Valaig.Data
@@ -12,37 +12,60 @@ namespace Valaig.Data
 /--
   `Pool α` is a memory pool data structure that allows storing, modifying, retrieving and freeing
   values referenced by unique `Nat` indices.
-
-  It is currently backed by `Std.HashMap`, but this may change in the future.
 -/
 structure Pool (α : Type) where
-  idx : Nat
-  values : Std.HashMap Nat α
-  ltIdx {idx' : Nat} : values.contains idx' → idx' < idx
-deriving Repr
+  values : Array α
+  frees : Std.HashSet Nat
+
+  freesValid : ∀ n ∈ frees, n < values.size
 
 namespace Pool
 variable {α : Type} {pool : Pool α} {idx idx' : Nat} {v : α}
+attribute [local simp, local grind →] Pool.freesValid
+attribute [local grind =] Std.HashSet.toList_iter
+attribute [local grind =_] Std.HashSet.mem_toList Std.Iter.getElem?_toList_eq_atIdxSlow?
 
-instance : Inhabited (Pool α) where
-  default := { idx := 0, values := .emptyWithCapacity, ltIdx := by grind }
+private theorem frees_perm :
+    pool.frees.iter.toList.Perm (List.range pool.values.size |>.filter (· ∈ pool.frees)) := by
+  simp only [Std.HashSet.toList_iter, List.perm_iff_count]
+  grind [List.Nodup.count, Std.HashSet.distinct_toList, List.count_filter]
+
+@[local simp, local grind =]
+private theorem rco_eq_range {n : Nat} :
+    (0...n).toList = List.range n := by
+  apply List.ext_get <;> simp
+
+@[local simp, local grind .]
+private theorem size_frees_le_size_values :
+    pool.frees.size ≤ pool.values.size := by
+  rw [show pool.frees.size = pool.frees.iter.toList.length by simp, List.Perm.length_eq frees_perm]
+  grind
+
+/--
+  The greatest number of elements that have been constructed up this point.
+  As indices are reused with a free list, indices from the free list are
+  guaranteed to be less than this.
+-/
+@[inline, local simp, local grind]
+def capacity (pool : Pool α) :=
+  pool.values.size
 
 @[inline]
 def contains (pool : Pool α) (idx : Nat) : Bool :=
-  pool.values.contains idx
+  idx < pool.capacity ∧ idx ∉ pool.frees
 
 instance instMembership : Membership Nat (Pool α) where
-  mem pool idx := idx ∈ pool.values
+  mem pool idx := pool.contains idx
 
 @[inline]
 instance {pool : Pool α} {idx : Nat} : Decidable (idx ∈ pool) := by
-  simp only [Membership.mem]
+  simp +instances only [instMembership]
   infer_instance
 
 @[local simp, local grind =]
-private theorem mem_eq :
-    (idx ∈ pool) = (idx ∈ pool.values) := by
-  rfl
+private theorem mem_iff :
+    idx ∈ pool ↔ idx < pool.capacity ∧ idx ∉ pool.frees := by
+  simp +instances [instMembership, contains]
 
 @[simp, grind =]
 theorem contains_eq_mem :
@@ -58,65 +81,32 @@ private theorem getElem_eq (h : idx ∈ pool) :
     pool[idx] = pool.values[idx] := by
   rfl
 
-@[inline]
-instance : GetElem? (Pool α) Nat α (fun pool idx => idx ∈ pool) where
-  getElem? pool idx := pool.values[idx]?
-
-@[local simp, local grind =]
-private theorem getElem?_eq :
-    pool[idx]? = pool.values[idx]? := by
-  rfl
-
-instance : LawfulGetElem (Pool α) Nat α (fun pool idx => idx ∈ pool) where
-  getElem?_def := by grind
-
 /--
-Returns the number of elements currently in the pool.
+  Return the number of elements currently in the pool.
 -/
 @[inline, local simp, local grind]
 def size (pool : Pool α) : Nat :=
-  pool.values.size
+  pool.capacity - pool.frees.size
 
 /--
-Returns a new index that is not currently valid within the pool. This can be used with `insert`
-to manually construct a new element in the pool.
+  Return a new index that is not currently valid within the pool. This can be used with `insert`
+  to manually construct a new element in the pool.
 -/
+@[inline]
 def nextIdx (pool : Pool α) : Nat :=
-  pool.idx
+  pool.frees.iter.atIdxSlow? 0 |>.getD pool.capacity
 
 @[simp, grind .]
 theorem nextIdx_not_in :
     pool.nextIdx ∉ pool := by
-  have := @pool.ltIdx
   grind [nextIdx]
 
 /--
-Creates an empty pool with memory allocated for `capacity` elements.
--/
-@[inline]
-def emptyWithCapacity (capacity : Nat := 8) : Pool α :=
-  {
-    idx := 0
-    values := .emptyWithCapacity capacity
-    ltIdx := by simp
-  }
-
-@[simp, grind .]
-theorem not_mem_emptyWithCapacity {cap : Nat} :
-    ¬(idx ∈ (emptyWithCapacity cap : Pool α)) := by
-  grind [emptyWithCapacity]
-
-@[simp, grind .]
-theorem size_emptyWithCapacity {cap : Nat} :
-    (emptyWithCapacity cap : Pool α).size = 0 := by
-  grind [emptyWithCapacity]
-
-/--
-Creates an empty pool with no memory allocated for elements.
+  Create an empty pool with no memory allocated for elements.
 -/
 @[inline]
 def empty : Pool α :=
-  .emptyWithCapacity 0
+  { values := #[], frees := .emptyWithCapacity, freesValid := by grind }
 
 @[simp, grind .]
 theorem not_mem_empty :
@@ -128,307 +118,264 @@ theorem size_empty :
     (empty : Pool α).size = 0 := by
   grind [empty]
 
-/--
-Adds a new element to the pool, returning the updated pool and a unique index for the new element.
--/
+@[simp, grind =]
+theorem capacity_empty :
+    (empty : Pool α).capacity = 0 := by
+  grind [empty]
+
 @[inline]
-def add (pool : Pool α) (v : α) : Pool α × Nat :=
-  ({
-    idx := pool.idx + 1
-    values := pool.values.insert pool.idx v
-    ltIdx := by have := @pool.ltIdx; grind
-  }, pool.idx)
+instance : Inhabited (Pool α) where
+  default := empty
 
-@[simp, grind =]
-theorem mem_add_iff :
-    idx ∈ (pool.add v).fst ↔
-      idx = (pool.add v).snd ∨ idx ∈ pool := by
-  grind [add]
-
-@[simp, grind .]
-theorem not_mem_add :
-    (pool.add v).snd ∉ pool := by
-  have := @pool.ltIdx
-  grind [add]
-
-@[simp, grind =]
-theorem getElem_add_self :
-    (pool.add v).fst[(pool.add v).snd] = v := by
-  grind [add]
-
-@[simp]
-theorem getElem_add (h : idx ∈ pool) :
-    (pool.add v).fst[idx] = pool[idx] := by
-  grind [add]
-
-grind_pattern getElem_add => (pool.add v).fst[idx] where
-  idx =/= (pool.add v).snd
-
-@[simp, grind =]
-theorem size_add :
-    (pool.add v).fst.size = pool.size + 1 := by
-  have : (pool.add v).snd ∉ pool := by grind
-  grind [add]
+section erase
+variable [Inhabited α]
 
 /--
-Adds a new `Inhabited.default` element to the pool, returning the updated pool and a unique index
-for the new element.
+  Remove an element from the pool by index.
 -/
 @[inline]
-def addD [Inhabited α] (pool : Pool α) : Pool α × Nat :=
-  pool.add Inhabited.default
-
-@[simp, grind =]
-theorem addD_eq [Inhabited α] :
-    pool.addD = pool.add Inhabited.default := by
-  rfl
-
-/--
-Removes an element from the pool by index. If there is no element allocated with that index, the
-pool is returned unchanged.
--/
-@[inline]
-def erase (pool : Pool α) (idx : Nat) : Pool α :=
-  { pool with
-    values := pool.values.erase idx
-    ltIdx := by have := @pool.ltIdx; grind
+def erase (pool : Pool α) (idx : Nat) (mem : idx ∈ pool := by grind) : Pool α :=
+  {
+    values := pool.values.set idx Inhabited.default
+    frees := pool.frees.insert idx
+    freesValid := by grind
   }
 
-@[simp, grind =]
-theorem mem_erase_iff :
-    idx ∈ (pool.erase idx') ↔
-      idx ≠ idx' ∧ idx ∈ pool := by
-  grind [erase]
+variable {mem : idx ∈ pool}
+attribute [local simp, local grind] erase
 
 @[simp, grind =]
-theorem getElem_erase (h : idx ∈ pool.erase idx') :
-    (pool.erase idx')[idx] = pool[idx] := by
-  grind [erase]
+theorem mem_erase_iff {idx' : Nat} :
+    idx' ∈ (pool.erase idx mem) ↔
+      idx' ≠ idx ∧ idx' ∈ pool := by
+  grind
+
+@[simp, grind =]
+theorem getElem_erase (h : idx' ∈ pool.erase idx mem) :
+    (pool.erase idx mem)[idx']'h = pool[idx'] := by
+  grind
 
 @[simp, grind =]
 theorem size_erase :
-    (pool.erase idx).size =
-    if idx ∈ pool then
-      pool.size - 1
-    else
-      pool.size := by
-  grind [erase]
+    (pool.erase idx mem).size = pool.size - 1 := by
+  grind
+
+@[simp, grind =]
+theorem capacity_erase :
+    (pool.erase idx mem).capacity = pool.capacity := by
+  grind
+
+end erase
 
 /--
-Inserts a new element at an index in the pool, growing the pool if needed. If the pool already
-contains an element at this index, it is overwritten.
+  Insert an element with index `nextIdx`.
 -/
 @[inline]
-def insert (pool : Pool α) (idx : Nat) (v : α) : Pool α :=
-  { idx := max pool.idx (idx + 1)
-    values := pool.values.insert idx v
-    ltIdx := by have := @pool.ltIdx; grind
-  }
+def push (pool : Pool α) (v : α) : Pool α :=
+  match h : pool.frees.iter.atIdxSlow? 0 with
+  | none => {
+      values := pool.values.push v
+      frees := pool.frees
+      freesValid := by grind
+    }
+  | some n => {
+      values := pool.values.set n v <| by apply pool.freesValid; grind
+      frees := pool.frees.erase n
+      freesValid := by grind
+    }
+
+section push
+attribute [local simp, local grind] push nextIdx
 
 @[simp, grind =]
-theorem mem_insert_iff :
-    idx ∈ pool.insert idx' v ↔
-      idx ∈ pool ∨ idx = idx' := by
-  grind [insert]
+theorem mem_push_iff :
+    idx ∈ pool.push v ↔
+      idx ∈ pool ∨ idx = pool.nextIdx := by
+  grind
 
 @[simp, grind =]
-theorem getElem_insert_self :
-    (pool.insert idx v)[idx] = v := by
-  grind [insert]
-
-@[simp]
-theorem getElem_insert (h : idx ∈ pool.insert idx' v) :
-    (pool.insert idx' v)[idx] =
-    if h : idx = idx' then
+theorem getElem_push (mem : idx ∈ pool.push v) :
+    (pool.push v)[idx]'mem =
+    if h : idx = pool.nextIdx then
       v
     else
       pool[idx] := by
-  grind [insert]
-
-grind_pattern getElem_insert => (pool.insert idx' v)[idx] where
-  idx =/= idx'
+  grind
 
 @[simp, grind =]
-theorem size_insert :
-    (pool.insert idx v).size =
-    if idx ∈ pool then
-      pool.size
-    else
-      pool.size + 1 := by
-  grind [insert]
-
-/--
-Replaces the element at a given index in the pool. See also `set?`.
--/
-@[inline]
-def set (pool : Pool α) (idx : Nat) (v : α) (h : idx ∈ pool := by get_elem_tactic) : Pool α :=
-  { pool with
-    values := pool.values.insert idx v
-    ltIdx := by have := @pool.ltIdx; grind
-  }
-
-@[simp, grind =]
-theorem mem_set_iff (h : idx' ∈ pool) :
-    idx ∈ (pool.set idx' v h) ↔ idx ∈ pool := by
-  grind [set]
-
-@[simp, grind =]
-theorem getElem_set_self (h : idx ∈ pool) :
-    (pool.set idx v h)[idx] = v := by
-  grind [set]
+theorem size_push :
+    (pool.push v).size = pool.size + 1 := by
+  grind [size_frees_le_size_values]
 
 @[simp]
-theorem getElem_set (h : idx ∈ pool) (h' : idx' ∈ pool) :
-    (pool.set idx' v h')[idx] =
-    if idx = idx' then
-      v
-    else
-      pool[idx] := by
-  grind [set]
+theorem capacity_push :
+    (pool.push v).capacity ≤ pool.capacity + 1 := by
+  grind
 
-grind_pattern getElem_set => (pool.set idx' v h')[idx] where
-  idx =/= idx'
+grind_pattern capacity_push => (pool.push v).capacity
 
-@[simp, grind =]
-theorem size_set (h : idx ∈ pool ) :
-    (pool.set idx v h).size = pool.size := by
-  grind [set]
+end push
 
+set_option linter.unusedVariables false in
 /--
-Replaces an element at the given index with the result of applying `f` to it. If there is no element
-allocated with that index, the pool is returned unchanged.
-
-The reference count to the element is decremented before applying `f`, allowing in-place updates.
+  Replace an element at the given index with the result of applying `f` to it.
+  The reference count to the element is decremented before applying `f`, allowing in-place updates.
 -/
 @[inline]
-def modify (pool : Pool α) (idx : Nat) (f : α -> α) : Pool α :=
+def modify (pool : Pool α) (idx : Nat) (f : α -> α) (mem : idx ∈ pool := by grind) : Pool α :=
   { pool with
     values := pool.values.modify idx f
-    ltIdx := by have := @pool.ltIdx; grind
+    freesValid := by grind
   }
 
-@[simp, grind =]
-theorem mem_modify_iff {f : α -> α} :
-    idx ∈ (pool.modify idx' f) ↔ idx ∈ pool := by
-  grind [modify]
+section modify
+variable {f : α -> α} {mem : idx ∈ pool}
+attribute [local simp, local grind] modify
 
 @[simp, grind =]
-theorem getElem_modify_self {f : α -> α} (h : idx ∈ pool) :
-    (pool.modify idx f)[idx] = f pool[idx] := by
-  grind [modify]
+theorem mem_modify_iff :
+    idx' ∈ (pool.modify idx f mem) ↔ idx' ∈ pool := by
+  grind
 
-@[simp]
-theorem getElem_modify {f : α -> α} (h : idx ∈ pool) :
-    (pool.modify idx' f)[idx] =
-    if idx = idx' then
-      f pool[idx]
+@[simp, grind =]
+theorem getElem_modify {mem' : idx' ∈ pool.modify idx f mem}:
+    (pool.modify idx f mem)[idx']'mem' =
+    if idx' = idx then
+      f pool[idx']
     else
-      pool[idx] := by
-  grind [modify]
-
-grind_pattern getElem_modify => (pool.modify idx' f)[idx] where
-  idx =/= idx'
+      pool[idx'] := by
+  grind
 
 @[simp, grind =]
-theorem size_modify {f : α -> α} :
+theorem size_modify :
     (pool.modify idx f).size = pool.size := by
-  grind [modify]
+  grind
 
+@[simp, grind =]
+theorem capacity_modify :
+    (pool.modify idx f).capacity = pool.capacity := by
+  grind
+
+end modify
+
+set_option linter.unusedVariables false in
 /--
-Replaces an element at the given index with the result of applying `f` to it, providing a proof that
-the element being modified matches the element visible to `GetElem?`.
-
-The reference count to the element is decremented before applying `f` by replacing the element with
-`Inhabited.default`, allowing in-place updates.
+  Move a value from an index into the pool to another index that is currently free or the same index,
+  resizing if required.
 -/
-@[inline]
-def modifyMem [Inhabited α] (pool : Pool α) (idx : Nat) (f : { elem : α // pool[idx]? = some elem } -> α)
-     (h : idx ∈ pool := by get_elem_tactic) : Pool α :=
-  let val := pool[idx]
-  let pool := pool.set idx Inhabited.default
-  pool.modify idx (fun _ => f ⟨val, by grind⟩)
+def move [Inhabited α] (pool : Pool α) (old new : Nat) (mem : old ∈ pool := by grind) (notmem : new ∉ pool ∨ new = old := by grind) : Pool α :=
+  if _ : new = old then
+    pool
+  else
+    -- Erase new from the free-list if needed and expand the array to have space
+    let pool : { p : Pool α // old < p.capacity ∧ new < p.capacity } :=
+      if _ : new < pool.capacity then
+        ⟨{ pool with
+          frees := pool.frees.erase new
+          freesValid := by grind
+        }, by grind⟩
+      else
+        let ⟨pool, _⟩ := resize pool
+        ⟨{ pool with
+          values := pool.values.push Inhabited.default
+          freesValid := by grind
+        }, by grind⟩
 
-@[simp, grind =]
-theorem mem_modifyMem_iff [Inhabited α] {f : { elem : α // pool[idx']? = some elem } -> α} (h : idx' ∈ pool) :
-    idx ∈ pool.modifyMem idx' f h ↔ idx ∈ pool := by
-  grind [modifyMem]
-
-@[simp, grind =]
-theorem getElem_modifyMem_self [Inhabited α] {f : { elem : α // pool[idx]? = some elem } -> α} (h : idx ∈ pool) :
-    (pool.modifyMem idx f h)[idx] = f ⟨pool[idx], by grind⟩ := by
-  grind [modifyMem]
-
-@[simp]
-theorem getElem_modifyMem [Inhabited α] {f : { elem : α // pool[idx']? = some elem } -> α} (h : idx ∈ pool) (h' : idx' ∈ pool) :
-    (pool.modifyMem idx' f h')[idx] =
-    if h : idx = idx' then
-      f ⟨pool[idx], by grind⟩
+    {
+      values := pool.val.values.swap old new
+      frees := pool.val.frees.insert old
+      freesValid := by grind
+    }
+where
+  -- Expand the array with freed default elements up to a size of new
+  resize (pool : Pool α) (size : pool.capacity ≤ new := by grind) : { p : Pool α // p.capacity = new } :=
+    if _ : pool.capacity = new then
+      ⟨pool, by grind⟩
     else
-      pool[idx] := by
-  grind [modifyMem]
+      resize {
+        values := pool.values.push Inhabited.default
+        frees := pool.frees.insert pool.capacity
+        freesValid := by grind
+      }
+  termination_by new + 1 - pool.capacity
+  decreasing_by grind
 
-grind_pattern getElem_modifyMem => (pool.modifyMem idx' f h')[idx] where
-  idx =/= idx'
+section move
+variable [Inhabited α] {old new : Nat} {mem : old ∈ pool} (notmem : new ∉ pool ∨ new = old) (size : pool.capacity ≤ new)
+attribute [local simp, local grind] move
 
 @[simp, grind =]
-theorem size_modifyMem [Inhabited α] {f : { elem : α // pool[idx]? = some elem } -> α} (h : idx ∈ pool) :
-    (pool.modifyMem idx f h).size = pool.size := by
-  grind [modifyMem]
+private theorem move.size_resize :
+    (move.resize new pool size).val.size = pool.size := by
+  fun_induction move.resize <;> grind
+
+@[simp, grind =]
+private theorem move.size_values_resize :
+    (move.resize new pool size).val.values.size = new := by
+  grind
+
+@[simp, grind =]
+private theorem move.size_frees_resize :
+    (move.resize new pool size).val.frees.size = pool.frees.size + (pool.capacity...new).size := by
+  fun_induction move.resize <;> grind [Nat.size_rco]
+
+@[simp, grind =]
+private theorem move.mem_resize :
+    idx ∈ (move.resize new pool size).val ↔ idx ∈ pool  := by
+  fun_induction move.resize <;> grind
+
+@[simp, grind =]
+private theorem move.mem_frees_resize :
+    idx ∈ (move.resize new pool size).val.frees ↔
+    idx ∈ pool.frees ∨
+    idx ∈ (pool.capacity...new) := by
+  fun_induction move.resize <;> grind [Std.Rco.mem_iff]
+
+@[simp, grind =]
+private theorem move.getElem_values_resize (mem : idx < (move.resize new pool size).val.values.size) mem' :
+    (move.resize new pool size).val.values[idx]'mem = pool[idx]'mem' := by
+  fun_induction move.resize <;> grind
+
+@[simp, grind =]
+theorem size_move :
+    (pool.move old new mem notmem).size = pool.size := by
+  simp only [move]
+  split
+  · grind
+  · split
+    · have : pool.frees.isEmpty = false := by grind [Std.HashSet.isEmpty_iff_forall_not_mem]
+      grind [Std.HashSet.isEmpty_eq_size_eq_zero]
+    · grind [Std.Rco.mem_iff, Nat.size_rco]
+
+@[simp, grind =]
+theorem capacity_move :
+    (pool.move old new mem notmem).capacity = max pool.capacity (new + 1) := by
+  grind
+
+@[simp, grind =]
+theorem mem_move :
+    idx ∈ pool.move old new mem notmem ↔
+    (idx ≠ old ∧ idx ∈ pool) ∨ idx = new := by
+  grind [Std.Rco.mem_iff]
+
+@[simp, grind =]
+theorem getElem_move (mem' : idx ∈ pool.move old new mem notmem) :
+    (pool.move old new mem notmem)[idx]'mem' =
+    if _ : idx = new then
+      pool[old]'mem
+    else
+      have h : idx ∈ pool := by grind
+      pool[idx]'h := by
+  grind
+
+end move
 
 /--
-Replaces the element at a given index in the pool. If there is no element allocated with that index,
-the pool is returned unchanged.
--/
-@[inline]
-def set? (pool : Pool α) (idx : Nat) (v : α) : Pool α :=
-  pool.modify idx (fun _ => v)
-
-@[simp, grind =]
-theorem mem_set?_iff :
-    idx ∈ (pool.set? idx' v) ↔ idx ∈ pool := by
-  grind [set?]
-
-@[simp, grind =]
-theorem getElem_set?_self (h : idx ∈ pool) :
-    (pool.set? idx v)[idx] = v := by
-  grind [set?]
-
-@[simp]
-theorem getElem_set? (h : idx ∈ pool) :
-    (pool.set? idx' v)[idx] =
-    if idx = idx' then
-      v
-    else
-      pool[idx] := by
-  grind [set?]
-
-grind_pattern getElem_set? => (pool.set? idx' v)[idx] where
-  idx =/= idx'
-
-@[simp, grind =]
-theorem size_set? :
-    (pool.set? idx v).size = pool.size := by
-  grind [set?]
-
-@[simp←]
-theorem size_zero_iff_forall_not_in :
-    pool.size = 0 ↔ ∀ (idx : Nat), idx ∉ pool := by
-  rw [show pool.size = 0 ↔ pool.values.isEmpty by grind [Std.HashMap.isEmpty_eq_size_eq_zero]]
-  simp [Std.HashMap.isEmpty_iff_forall_contains]
-
-grind_pattern size_zero_iff_forall_not_in => (_ : Nat) ∈ pool, pool.size
-
-@[expose, reducible]
-def IterState (pool : Pool α) : Type :=
-  let getType {α β} (_ : @Std.Iter α β) := α
-  getType pool.values.keysIter
-
-/--
-Returns an iterator over the valid indices in the pool.
+  Return an iterator over the valid indices in the pool.
 -/
 @[inline]
 def iter (pool : Pool α) :=
-  pool.values.keysIter
+  (0...pool.values.size).iter.filter (· ∉ pool.frees)
 
 @[simp, grind =]
 theorem mem_iter_toList_iff_mem :
@@ -438,7 +385,12 @@ theorem mem_iter_toList_iff_mem :
 @[simp, grind =]
 theorem length_iter_eq_size :
     pool.iter.length = pool.size := by
-  simp [iter, ←Std.Iter.length_toList_eq_length]
+  simp only [iter, ← Std.Iter.length_toList_eq_length, Std.Iter.toList_filter, ← List.countP_eq_length_filter]
+  have {α : Type} {l : List α} f : l.countP f = l.length - l.countP (!f ·) := by grind [List.length_eq_countP_add_countP]
+  rw [this, Std.Rco.toList_iter, Std.Rco.length_toList]
+  congr 1
+  rw [show pool.frees.size = pool.frees.iter.toList.length by simp, List.Perm.length_eq frees_perm]
+  grind
 
 @[simp, grind =]
 theorem length_toList_iter :
@@ -448,7 +400,9 @@ theorem length_toList_iter :
 @[simp, grind .]
 theorem nodup_toList_iter :
     pool.iter.toList.Nodup := by
-  simp [iter, Std.HashMap.nodup_keys]
+  simp only [List.Nodup, iter, Std.Iter.toList_filter, List.pairwise_filter]
+  apply List.Pairwise.imp ?_ Std.Rco.pairwise_toList_ne
+  grind
 
 theorem distinct_toList_iter {idx idx' : Nat} (h : idx < pool.size) (h' : idx' < pool.size)
     (diff : idx ≠ idx') :
